
Consider the simplest case, with two binary variables \(Z\) and \(K\). We fit the model

\[
  E(Y|Z,K) = \beta_0 + \beta_1Z + \beta_2K + \beta_3ZK,
\]

where \(ZK = 1\) only if both \(Z = 1\) and \(K = 1\).

This is functionally equivalent to defining a new variable \(L\),

\[
  L = \begin{cases}
  0, & K = 0\ \&\ Z = 0 \\
  1, & K = 0\ \&\ Z = 1 \\
  2, & K = 1\ \&\ Z = 0 \\
  3, & K = 1\ \&\ Z = 1,
  \end{cases}
\]

and fitting the model

\[
  E(Y|L) = \beta_0 + \beta_1l_1 + \beta_2l_2 + \beta_3l_3.
\]
